qed: point add 8

code/ecdsap256/Hacl.Impl.P256.PointAdd8.fst
@@ -17,8 +17,10 @@ open FStar.Mul
 
 open Hacl.Impl.P256.Core
 open Hacl.Impl.P256.PointAdd
+open Hacl.Impl.P256.LowLevel
 
 friend Hacl.Impl.P256.Core
+
 
 #set-options "--z3rlimit 150 --ifuel 0 --fuel 0" 
 
@@ -45,3 +47,137 @@ let _point_add8 p q result tempBuffer =
   pointToDomain q q;
   point_add p q result tempBuffer;
   norm result result tempBuffer
+
+
+val toForm: i: lbuffer uint8 (size 32) -> o: felem -> Stack unit
+  (requires fun h -> live h i /\ live h o /\ disjoint i o /\ Lib.ByteSequence.nat_from_bytes_be (as_seq h i) < prime256)
+  (ensures  fun h0 _ h1 -> modifies (loc o) h0 h1 /\ 
+    as_nat h1 o == Lib.ByteSequence.nat_from_bytes_be (as_seq h0 i) /\
+    as_nat h1 o < prime)
+
+let toForm i o = 
+  let open Lib.ByteSequence in 
+    let h0 = ST.get() in 
+  toUint64ChangeEndian i o;
+    let h1 = ST.get() in 
+  lemma_core_0 o h1;
+  Spec.ECDSA.changeEndianLemma (uints_from_bytes_be (as_seq h0 i));
+  uints_from_bytes_be_nat_lemma #U64 #_ #4 (as_seq h1 i)
+
+inline_for_extraction noextract
+val toFormPoint: p: lbuffer uint8 (size 64) -> o: point -> Stack unit 
+  (requires fun h -> live h p /\ live h o /\ disjoint p o /\ (
+    let pX = gsub p (size 0) (size 32) in 
+    let pY = gsub p (size 32) (size 32) in 
+    Lib.ByteSequence.nat_from_bytes_be (as_seq h pX) < prime256 /\
+    Lib.ByteSequence.nat_from_bytes_be (as_seq h pY) < prime256))
+  (ensures fun h0 _ h1 -> modifies (loc o) h0 h1 /\ (
+    let pX, pY = gsub p (size 0) (size 32), gsub p (size 32) (size 32) in
+    let rX, rY, rZ = gsub o (size 0) (size 4),  gsub o (size 4) (size 4), gsub o (size 8) (size 4) in 
+
+    as_nat h1 rX == Lib.ByteSequence.nat_from_bytes_be (as_seq h0 pX) /\
+    as_nat h1 rY == Lib.ByteSequence.nat_from_bytes_be (as_seq h0 pY) /\
+
+    (as_nat h1 rX, as_nat h1 rY, as_nat h1 rZ) == 
+      Spec.P256.toJacobianCoordinates (Lib.ByteSequence.nat_from_bytes_be (as_seq h0 pX), Lib.ByteSequence.nat_from_bytes_be (as_seq h0 pY)) /\
+    as_nat h1 rX < prime /\ as_nat h1 rY < prime /\ as_nat h1 rZ == 1))
+
+let toFormPoint i o = 
+  let pU64X = sub o (size 0) (size 4) in
+  let pU64Y = sub o (size 4) (size 4) in
+  let pX = sub i (size 0) (size 32) in
+  let pY = sub i (size 32) (size 32) in
+
+  toForm pX pU64X;
+  toForm pY pU64Y;
+  Hacl.Impl.P256.Signature.Common.bufferToJacUpdate o
+
+
+
+inline_for_extraction noextract
+val fromForm: i: felem -> o: lbuffer uint8 (size 32) -> Stack unit 
+  (requires fun h -> live h i /\ live h o /\ disjoint i o /\ as_nat h i < prime256)
+  (ensures fun h0 _ h1 -> modifies (loc i |+| loc o) h0 h1 /\  
+    as_seq h1 o == Lib.ByteSequence.nat_to_bytes_be 32 (as_nat h0 i))
+
+
+let fromForm i o = 
+  let open Lib.ByteSequence in 
+  let h0 = ST.get() in
+  changeEndian i;
+    let h1 = ST.get() in 
+  toUint8 i o;
+  lemma_core_0 i h0;
+  lemma_nat_from_to_intseq_le_preserves_value 4 (as_seq h0 i);
+  Spec.ECDSA.changeEndian_le_be (as_nat h0 i)
+
+
+inline_for_extraction noextract
+val fromFormPoint: i: point -> o: lbuffer uint8 (size 64) -> Stack unit 
+  (requires fun h -> live h i /\ live h o /\ disjoint i o /\ (
+    let iX = gsub i (size 0) (size 4) in 
+    let iY = gsub i (size 4) (size 4) in 
+    as_nat h iX < prime256 /\ as_nat h iY < prime256))
+  (ensures fun h0 _ h1 -> modifies (loc i |+| loc o) h0 h1 /\ (
+    let iX = gsub i (size 0) (size 4) in 
+    let iY = gsub i (size 4) (size 4) in 
+
+    let oX = gsub o (size 0) (size 32) in 
+    let oY = gsub o (size 32) (size 32) in 
+
+    as_seq h1 oX == Lib.ByteSequence.nat_to_bytes_be 32 (as_nat h0 iX) /\ 
+    as_seq h1 oY == Lib.ByteSequence.nat_to_bytes_be 32 (as_nat h0 iY)))
+
+let fromFormPoint i o = 
+  let iX = sub i (size 0) (size 4) in 
+  let iY = sub i (size 4) (size 4) in 
+
+  let oX = sub o (size 0) (size 32) in 
+  let oY = sub o (size 32) (size 32) in 
+
+  fromForm iX oX;
+  fromForm iY oY
+
+
+val point_add8: result: lbuffer uint8 (size 64) -> p: lbuffer uint8 (size 64) -> q: lbuffer uint8 (size 64) -> 
+  Stack unit 
+  (requires fun h -> live h result /\ live h p /\ live h q /\ (
+    let pX = gsub p (size 0) (size 32) in 
+    let pY = gsub p (size 32) (size 32) in 
+    let qX = gsub q (size 0) (size 32) in 
+    let qY = gsub q (size 32) (size 32) in
+    
+    Lib.ByteSequence.nat_from_bytes_be (as_seq h pX) < prime256 /\ 
+    Lib.ByteSequence.nat_from_bytes_be (as_seq h pY) < prime256 /\
+    Lib.ByteSequence.nat_from_bytes_be (as_seq h qX) < prime256 /\
+    Lib.ByteSequence.nat_from_bytes_be (as_seq h qY) < prime256))
+  (ensures fun h0 _ h1 -> modifies (loc result) h0 h1 /\ (
+    let open Lib.ByteSequence in 
+    let pX = nat_from_bytes_be (as_seq h0 (gsub p (size 0) (size 32))) in 
+    let pY = nat_from_bytes_be (as_seq h0 (gsub p (size 32) (size 32))) in
+    let pK = Spec.P256.toJacobianCoordinates (pX, pY) in 
+    
+    let qX = nat_from_bytes_be (as_seq h0 (gsub q (size 0) (size 32))) in 
+    let qY = nat_from_bytes_be (as_seq h0 (gsub q (size 32) (size 32))) in
+    let qK = Spec.P256.toJacobianCoordinates (qX, qY) in 
+    let resultX, resultY, _ = Spec.P256._norm (Spec.P256._point_add pK qK) in 
+    
+    as_seq h1 (gsub result (size 0) (size 32)) == nat_to_bytes_be 32 resultX /\
+    as_seq h1 (gsub result (size 32) (size 32)) == nat_to_bytes_be 32 resultY))
+
+
+let point_add8 result p q = 
+  push_frame();
+    let tempBuffer = create (size 124) (u64 0) in 
+  
+    let pU64 = sub tempBuffer (size 0) (size 12) in 
+    let qU64 = sub tempBuffer (size 12) (size 12) in 
+    let resultU64 = sub tempBuffer (size 24) (size 12) in 
+    let tB88 = sub tempBuffer (size 36) (size 88) in 
+
+    toFormPoint p pU64; 
+    toFormPoint q qU64;
+    _point_add8 pU64 qU64 resultU64 tB88;
+    fromFormPoint resultU64 result;
+
+  pop_frame()
